Thought about changing it to a new layout

model/noc.dfy
@@ -1,16 +1,81 @@
-include "router.dfy"
+module NoC {
+  type Length = i: nat | 1 <= i witness 1
 
-type Noc = seq<seq<Router>>
+  const BUFFER_LENGTH: Length
 
-ghost predicate Valid(n: Noc)
-{
-  && |n| >= 2
-  && (forall i :: 0 <= i < |n| ==> |n[i]| == |n|)
-  && (forall i, j :: 0 <= i < |n| && 0 <= j < |n| ==> n[i][j].id == i*|n| + j)
-}
+  datatype Buffer<T> =
+    | Node(payload: T, next: Buffer)
+    | Tail
+    {
+      function length(): nat {
+        match this
+        case Node(_, next) => 1 + next.length()
+        case Tail => 0
+      }
 
-ghost predicate containsId(n: Noc, id: Id)
-  requires Valid(n)
-{
-  exists i, j :: n[i][j].id == id
+      function append(p: T): Buffer<T> {
+        match this
+        case Node(payload, next) => Node(payload, next.append(p))
+        case Tail => Node(p, Tail)
+      }
+    }
+
+  datatype Direction =
+    | North
+    | South
+    | East
+    | West
+    | Local
+
+  class Router<T> {
+    var North: Buffer<T>
+    var East:  Buffer<T>
+    var South: Buffer<T>
+    var West:  Buffer<T>
+    var Local: Buffer<T>
+
+    constructor()
+      ensures North.length() == 0 && East.length() == 0 && South.length() == 0 && West.length() == 0 && Local.length() == 0
+    {
+      North := Tail;
+      South := Tail;
+      East  := Tail;
+      West  := Tail;
+      Local := Tail;
+    }
+
+    method insertLocal(payload: T)
+      modifies this.Local 
+    {
+      this.Local := this.Local.append(payload);
+    }
+  }
+
+  type NoC = n: seq<seq<Router<nat>>> | |n| >= 2 && (forall y :: 0 <= y < |n| ==> |n[y]| == |n|) witness *
+
+  method generateFlits(n: NoC, cycle: nat) returns (n': NoC)
+  {
+    n' := n;
+
+    if cycle % 3 >= 3 {
+      return;
+    }
+
+    var dim := |n|;
+    var y := 0;
+
+    while y < dim
+    {
+      var x := 0;
+      while x < dim
+      {
+        if n'[y][x].Local.length() < BUFFER_LENGTH {
+          var dest_id :| 0 <= dest_id < dim * dim && dest_id != y*dim + x;
+          n'[y][x].Local := n'[y][x].Local.append(dest_id);
+        }
+        x := x + 1;
+      }
+      y := y + 1;
+    }
+  }
 }
