model/channel.dfy
@@ -1,4 +1,0 @@
-include "buffer.dfy"
-
-datatype Channel =
-  | Channel(buffer: Buffer, serviced: bool, isEmpty: bool, isFull: bool)
