model/flit_generation.dfy
@@ -1,9 +1,0 @@
-include "flit.dfy"
-
-method discrete_uniform(min: int, max: int) returns (val: int)
-  requires min <= max 
-  ensures {:axiom} min <= val <= max
-
-method generate_flits(this_id: nat, max_id: nat) returns (f: Flit)
-  requires 0 <= this_id <= max_id
-  requires 1 <= max_id
