model/id.dfy
@@ -1,5 +1,0 @@
-type Id = nat
-
-datatype ConnectId = 
-  | Id(id: Id)
-  | NoConnect
